![image-20210307192941047](C:\Users\Joshua\AppData\Roaming\Typora\typora-user-images\image-20210307192941047.png)

## (i)

### since for $\forall\ x\ P(x) = \prod_{i=1}^{n}\ (x-e_i)\ - \prod_{i=1}^{n}(x-e_i')=0$ , take $x=[e_1,...,e_{n_i}]$ , get $x$ must equal to one of $[e'_1,..,e'_{n_i}]$ , so for $e \in [e_1,...,e_{n_i}]$, $e$ is equal to one of $[e'_1,..,e'_{i}]$, so $[e_1,...,e_{n_i}]$ is a permutation of  $[e'_1,..,e'_{i}]$.

## (ii)

### the polynomial $P(x) = \prod_{i=1}^{n}\ (x-e_i)\ - \prod_{i=1}^{n}(x-e_i')$ is of degree $n-1$, so according to the theorem, there are at most $n-1$ zeros, so the probability is $\frac{n-1}{p}$;

### And since we can find one solution of these $n-1$ zeros by assigning that $e_i=e'_i$ except $e_n\not=e'_n$ since $[e_1,...,e_{n_i}]$ is not the permutation of $[e'_1,..,e'_{n_i}]$ .

### in this way, we can take 

### 																				$e_{max}=n-1$, 

### so  we get 														$p>Max[\frac{n}{\varepsilon},n-1]$ 

### so we get														$P=\frac{n-1}{p}<\frac{n-1}{n}{\varepsilon}<{\varepsilon}$

### when $n$ goes to $\infin$ , $p=\varepsilon$

### 

