## Exercise 1

(i)


$$
\begin{aligned}
&{\rm sorted\_list} \leftarrow sort({\rm unsorted\_list}) =\\
&\qquad	\boldsymbol{{\rm IF}}\ {\rm sorted\_list} = undef \\
&\qquad	\boldsymbol{\rm{THEN\ LET}}\ n = length({\rm unsorted\_list}) \\
&\qquad\qquad	\boldsymbol{\rm{IN\ PAR}} \\
&\qquad\qquad\qquad	\boldsymbol{\rm{IF}}\ {\rm sorted\_list_1} = undef\ \wedge\ ...\ \wedge\ {\rm sorted\_list_k} = undef \\
&\qquad\qquad\qquad		\boldsymbol{\rm THEN\ LET}\ {\rm list_1} = \boldsymbol{\rm I} L_1.length(L_1) = \lceil\frac nk\rceil)\wedge\exist{L'}.concat(L_1,L') = {\rm unsorted\_list} \\ 
&\qquad\qquad\qquad\qquad\boldsymbol{\rm IN\ \ \ \ LET}\ list_2 = \boldsymbol{\rm I}L_2.length(L_2) = \lceil \frac{n-\sum^1_{i=1}|L_i|}{k-1}\rceil\wedge \exist L'.concat(L_1,L_2,L') = {\rm unsorted\_list}\\
&\qquad\qquad\qquad\qquad\qquad \bold{IN} \ldots \\
&\qquad\qquad\qquad\qquad\qquad\qquad\qquad \bold{IN\ LET}\ list_k= \bold{I}L_k.length(L_k) = \lceil \frac{n-\sum^{k-1}_{i=1}|L_i|}{1}\rceil\wedge \exist L'.concat(L_1,L_2,L') = {\rm unsorted\_list}\\
&\qquad\qquad\qquad\qquad\qquad\qquad\qquad\qquad \bold{IN\ PAR} {\rm \ sorted\_list_1} = sort({\rm list_1}) \\
&\qquad\qquad\qquad\qquad\qquad\qquad\qquad\qquad\qquad\qquad\qquad\qquad \ldots\\
&\qquad\qquad\qquad\qquad\qquad\qquad\qquad\qquad\qquad\qquad\;\:\! {\rm sorted\_list_k} = sort({\rm list_k})\\
&\qquad\qquad\qquad\qquad\qquad\qquad\qquad\qquad\bold{ENDPAR}\\
&\qquad\qquad\qquad\bold{ENDIF}\\
&\qquad\qquad\qquad\bold{IF}\ {\rm sorted\_list_1} \neq undef \wedge \ldots \wedge {\rm sorted\_list_k} \neq undef\\
&\qquad\qquad\qquad\bold{THEN}\ {\rm sorted\_list} \leftarrow merge({\rm sorted\_list_1,\ldots,sorted\_list_k})\ \bold{ENDIF} \\
&\qquad\qquad\bold{ENDPAR}\\
&\qquad\bold{ENDIF}
\end{aligned}
$$

$$
\begin{aligned}
&{\rm merged\_list} \leftarrow merge({\rm inlist_1, \ldots, inlist_k})\\
& \bold{IF}\ {\rm merged\_list} = undef\ \bold{THEN}\\
& \qquad \bold{LET}\ x_1 = head({\rm inlist_1),\ restlist_1} = tail({\rm inlist_1}),\\
& \qquad\qquad\qquad \ldots \\
& \qquad\qquad\:\; x_k = head({\rm inlist_k}),\ {\rm restlist_k} = tail({\rm inlist_k})\ \bold{IN\ PAR}\\
& \qquad\qquad \bold{IF}\ x_1 \leq \forall x_i.\{i\neq 1\} \wedge {\rm merged\_restlist}=undef\\
& \qquad\qquad \bold{THEN}\ {\rm merged\_restlist} \leftarrow merge({\rm restlist_1,inlist_2,\ldots,inlist_k}) \ \bold{ENDIF}\\
& \qquad\qquad \bold{IF}\ x_2 \leq \forall x_i.\{i\neq 2\} \wedge {\rm merged\_restlist} = undef \\
& \qquad\qquad \bold{THEN}\ {\rm merged\_restlist} \leftarrow merge({\rm inlist_1,restlist_2,inlist_3,\ldots,inlist_k}) \ \bold{ENDIF}\\
& \qquad\qquad\qquad \ldots \\
& \qquad\qquad \bold{IF}\ x_k \leq \forall x_i.\{i\neq k\} \wedge {\rm merged\_restlist} = undef \\
& \qquad\qquad \bold{THEN}\ {\rm merged\_restlist} \leftarrow merge({\rm inlist_1,\ldots, inlist_{k-1},restlist_k})\ \bold{ENDIF}\\

& \qquad\qquad \bold{IF}\ x_1 \leq \forall x_i.\{i\neq 1\} \wedge {\rm merged\_restlist}\neq undef\\
& \qquad\qquad \bold{THEN}\ {\rm merged\_list} := concat([x_1], {\rm merged\_restlist})\ \bold{ENDIF}\\
& \qquad\qquad \bold{IF}\ x_2 \leq \forall x_i.\{i\neq 2\} \wedge {\rm merged\_restlist} \neq undef \\
& \qquad\qquad \bold{THEN}\ {\rm merged\_list} := concat([x_2], {\rm merged\_restlist})\ \bold{ENDIF}\\
& \qquad\qquad\qquad \ldots \\
& \qquad\qquad \bold{IF}\ x_k \leq \forall x_i.\{i\neq k\} \wedge {\rm merged\_restlist} \neq undef \\
& \qquad\qquad \bold{THEN}\ {\rm merged\_list} := concat([x_k], {\rm merged\_restlist})\ \bold{ENDIF}\\
& \qquad \bold{ENDPAR}\\
& \bold{ENDIF}
\end{aligned}
$$

**Note:** For the simplicity of expression of the algorithm, we omit the case where $n < thr $  in the original binomial mergesort algorithm.



Complexity Analysis:

â€‹	First we see that for the merge algorithm, its complexity is in $\Theta(n)$.  (We omit the complexity analysis when $n < thr$ since it is trivial.) 
$$
f(n) = f(\lfloor{\frac nk}\rfloor) + f(\lfloor{\frac nk}\rfloor) + \ldots+f(n - (k-1) * \lfloor{\frac nk}\rfloor) + g(n) + d < k*f(\lfloor{\frac nk}\rfloor) + g(n) + d
$$
Replacing $n$ by $k^n$ this leads to a linear recurrence relation,
$$
h_n - k\cdot h_{n-1} = a_2\cdot k^n + b_2 + d
$$
 The characteristic polynomial is $(x-k)^2(x-1)$, which gives rise to 
$$
h_n = c_1 \cdot k^n + c_2 \cdot n\cdot k^n + c_3
$$
 and further 
$$
f_n = c_1 \cdot n + c_2\cdot \log_k(n)\cdot n + c_3 \in O(n\log(n) | \varphi(n))
$$
where the condition $\varphi(n)$ express that $n$ is a power of $k$.

As $n\log(n)$ is smooth and monotone increasing (almost everywhere), we can infer that $f_n \in O(n\log(n))$. 

And further because of the lower complexity bound of comparison-based sorting algorithm, $f_n \in \Theta(n\log{n})$. 



Finally we have shown that the complexity of the generalized Mergesort has invariant complexity under $k$.



